{
 "cells": [
  {
   "cell_type": "markdown",
   "id": "b83c0460-f5f5-4dba-9fa1-21846f256b0b",
   "metadata": {},
   "source": [
    "## Algebric Identities\n",
    "\n",
    "---\n",
    "\n",
    "$ \\qquad\\qquad\\begin{equation*} \\left(a \\pm b \\right)^2=a^2+b^2 \\pm 2ab = \\left\\{\\begin{array}{rl}  \\left(a+b \\right)^2=a^2+b^2+2ab \\\\ \\left(a-b \\right)^2=a^2+b^2-2ab \\end{array} \\right. \\end{equation*} $\n",
    "\n",
    "---\n",
    "\n",
    "$ \\qquad\\qquad \\begin{equation*} \\begin{aligned}\n",
    "\\left(a+b \\right)^2=a^2+b^2+2ab \\Rightarrow a^2+b^2=\\left(a+b \\right)^2 - 2ab  \\\\\n",
    "\\left(a-b \\right)^2=a^2+b^2-2ab \\Rightarrow a^2+b^2=\\left(a-b \\right)^2 + 2ab \\end{aligned} \\end{equation*} $  \n",
    "$\\qquad\\qquad\\qquad\\qquad\\qquad\\qquad\\qquad\\quad(+)$                                                                                                     \n",
    "$\\qquad\\qquad\\qquad\\qquad$_________________________________________________________________________                                       \n",
    "$\\qquad\\qquad\\qquad\\qquad\\qquad\\qquad\\qquad \\ \\ \\ \\begin{aligned}  2\\left(a^2+b^2 \\right) &= \\left(a+b \\right)^2 + \\left(a-b \\right)^2 \\\\  \\left(a^2+b^2 \\right) &= \\frac{\\left(a+b \\right)^2}{2} + \\frac{\\left(a-b \\right)^2}{2} \\\\  \\left(a^2+b^2 \\right) &= \\left( \\frac{a+b}{\\sqrt{2}} \\right)^2 + \\left( \\frac{a-b}{\\sqrt{2}} \\right)^2 \\end{aligned}$  \n",
    "\n",
    "---\n",
    "\n",
    "$ \\qquad\\qquad \\begin{equation*} \\begin{aligned}\n",
    "\\left(a+b \\right)^2=a^2+b^2+2ab \\Rightarrow a^2+b^2=\\left(a+b \\right)^2 - 2ab  \\\\\n",
    "\\left(a-b \\right)^2=a^2+b^2-2ab \\Rightarrow a^2+b^2=\\left(a-b \\right)^2 + 2ab \\end{aligned} \\end{equation*} $  \n",
    "$\\qquad\\qquad\\qquad\\qquad\\qquad\\qquad\\qquad\\quad(-)$                                                                                                                \n",
    "$\\qquad\\qquad\\qquad\\qquad$_________________________________________________________________________                                       \n",
    "$\\qquad\\qquad\\qquad\\qquad\\qquad\\qquad\\qquad\\qquad\\quad \\ \\ \\begin{aligned} 0 &= \\left(a+b \\right)^2 - \\left(a-b \\right)^2 - 4ab \\\\ 4ab &= (a + b)^2 - (a - b)^2 => \\left\\{\\begin{array}{rl}  \\left(a+b \\right)^2= \\left(a-b \\right)^2 + 4ab \\\\ \\left(a-b \\right)^2= \\left(a+b \\right)^2 - 4ab \\end{array} \\right. \\\\ ab &= \\frac{(a + b)^2}{4} - \\frac{(a - b)^2}{4} \\\\ ab &= \\left(\\frac{a + b}{2} \\right)^2 - \\left(\\frac{a - b}{2} \\right)^2 \\end{aligned}$                                       \n",
    "\n",
    "---\n",
    "\n",
    "$\\qquad\\qquad a^2-b^2 = a^2 - ab + ab - b^2 = a(a-b) + b(a-b) = (a-b)(a+b) $\n",
    "\n",
    "---\n",
    "\n",
    "$\\qquad\\qquad (a+b+c)^2 = a^2+b^2+c^2 + 2(ab+bc+ac)$                                                                                                                      \n",
    "$\\qquad\\qquad a^2+b^2+c^2  = (a+b+c)^2 - 2(ab+bc+ac)$\n",
    "\n",
    "---\n",
    "\n",
    "$  \\qquad\\qquad\\begin{equation*} \\left(a \\pm b \\right)^3=a^3 \\pm b^3 \\pm 3ab(a \\pm b) = \\left\\{\\begin{array}{rl}  \\left(a+b \\right)^3=a^3+b^3+3ab(a+b) \\\\ \\left(a-b \\right)^3=a^3-b^3-3ab(a-b) \\end{array} \\right. \\end{equation*} $\n",
    "\n",
    "---\n",
    "\n",
    "$ \\qquad\\qquad (a^3+b^3) = (a+b)^3 - 3ab(a+b)= (a+b)\\left\\{ (a+b)^2-3ab \\right\\} = (a+b)\\left\\{ a^2+b^2+2ab-3ab \\right\\}=(a+b)(a^2+b^2-ab )$\n",
    "\n",
    "$ \\qquad\\qquad (a^3-b^3) = (a-b)^3 + 3ab(a-b)= (a-b)\\left\\{ (a-b)^2+3ab \\right\\} = (a-b)\\left\\{ a^2+b^2-2ab+3ab \\right\\}=(a-b)(a^2+b^2+ab )$\n",
    "\n",
    "---\n",
    "\n",
    "$ \\qquad\\qquad \\begin{aligned} (a + b + c)^3 &= (a + b + c)(a + b + c)(a + b + c) \\\\ &= (a + b + c)(a^2+b^2+c^2 + 2ab+ 2bc + 2ac) \\\\\n",
    "&= a(a^2+b^2+c^2 + 2ab+ 2bc + 2ac) + b(a^2+b^2+c^2 + 2ab+ 2bc + 2ac) + c(a^2+b^2+c^2 + 2ab+ 2bc + 2ac) \\\\\n",
    "&= a^3 + ab^2 + ac^2 + 2a^2b + 2abc + a^2b + b^3 + bc^2 + 2ab^2 + 2b^2c + 2abc + a^2c + b^2c + c^3 + 2abc + 2bc^2 + 2ac^2 \\\\\n",
    "&= a^3 + b^3 + c^3 + 3a^2b + 3ab^2 + 3a^2c + 3ac^2 + 3b^2c + 3bc^2 + 6abc \\\\\n",
    "&= a^3 + b^3 + c^3 + 3(a^2b + ab^2 + b^2c + bc^2 + c^2a + ca^2) + 6abc \\\\\n",
    "&= a^3 + b^3 + c^3 + 3[ ab(a+b) + bc(b+c) + ca(c+a) ] + 6abc  \\\\\n",
    "&= a^3 + b^3 + c^3 + 3[ ab(a+b) + bc(b+c) + ca(c+a) + 2abc ] \\\\\n",
    "&= a^3 + b^3 + c^3 + 3(a + b)(b + c)(c + a)  \\end{aligned} $\n",
    "\n",
    "$ \\qquad\\qquad \\begin{aligned} (a + b + c)^3  - (a^3 + b^3 + c^3) = 3(a + b)(b + c)(c + a)  \\end{aligned} $ \n",
    "\n",
    "$ \\qquad\\qquad \\begin{aligned} a^3 + b^3 + c^3 - 3abc &=  (a + b)^3 - 3ab(a + b) + c^3 - 3abc \\\\\n",
    "&=  (a + b)^3 + c^3 - 3ab(a + b) - 3abc \\qquad\\qquad\\qquad\\qquad\\qquad [\\because \\ \\text{arranging}] \\\\\n",
    "&=  (a + b)^3 + c^3 - 3ab(a + b + c) \\qquad\\qquad\\qquad\\qquad\\qquad\\quad \\ [\\because \\ \\text{taking common }-3ab]  \\\\\n",
    "&= (a + b + c)\\{(a+b)^2-(a+b)c+c^2\\} - 3ab(a + b + c) \\\\\n",
    "&= (a + b + c)\\{a^2+b^2+2ab-ac-bc+c^2\\} - 3ab(a + b + c) \\\\\n",
    "&= (a + b + c)(a^2+b^2+2ab-ac-bc+c^2 - 3ab) \\qquad\\qquad\\qquad [\\because \\ \\text{taking common }(a+b+c)]  \\\\\n",
    "&= (a + b + c)(a^2 + b^2 + c^2 - ab - bc - ca) \\qquad\\qquad\\qquad\\qquad\\quad [\\because \\ \\text{arranging}] \\\\\n",
    "&= (a + b + c) \\ \\frac{1}{2}\\times 2 \\ (a^2 + b^2 + c^2 - ab - bc - ca) \\\\\n",
    "&= \\frac{1}{2} (a + b + c) (2a^2 + 2b^2 + 2c^2 - 2ab - 2bc - 2ca) \\\\\n",
    "&= \\frac{1}{2} (a + b + c) [(a^2 + b^2 - 2ab) + (b^2 + c^2- 2bc) + (c^2 + a^2 - 2ca)] \\\\\n",
    "&= \\frac{1}{2} (a + b + c) [(a-b)^2+(b-c)^2+(c-a)^2] \\\\ \n",
    "\\end{aligned} $\n",
    "\n",
    "---"
   ]
  },
  {
   "cell_type": "markdown",
   "id": "cc93703b-70c8-4cf6-82de-13b5751ea563",
   "metadata": {},
   "source": [
    "## Interest \n",
    "\n",
    "$\\text{S.I.} = \\frac{P\\times T\\times r}{100} $\n",
    "\n",
    "$\\text{C.I.} = P\\left[\\left(1+\\frac{r}{100\\times n} \\right)^{nt} -1\\right]$\n",
    "\n",
    "$ A = P\\left(1+\\frac{r}{100\\times n} \\right)^{nt}$\n",
    "\n",
    "For time=2yrs : $ C.I. - S.I. =P\\times \\left(\\frac{r}{100}\\right)^2$\n",
    "\n",
    "For time=3yrs : $ C.I. - S.I. =P\\times \\left(\\frac{r}{100}\\right)^2 \\times\\left(\\frac{r}{100} + 3\\right)$"
   ]
  },
  {
   "cell_type": "markdown",
   "id": "c2861b89-df49-4282-8f0a-90b59b2ea3ac",
   "metadata": {},
   "source": [
    "## Statistics \n",
    "\n",
    "Mean $ \\displaystyle\\bar{x}=\\frac{\\sum{x_{\\tiny{i}}}}{n}=\\frac{ \\sum{ f_{\\tiny{i}} x_{\\tiny{i}} } } {\\sum f_{\\tiny{i}}}$\n",
    "\n",
    "$\\displaystyle \\begin{equation*} \\text{Median} = \\left\\{\\begin{array}{rl} \\frac{(n+1)}{2}th\\text{ term} & \\text{if } n \\text{ is odd}, \\\\  \\left[\\frac{\\frac{n}{2}th\\text{ term} + \\frac{(n+1)}{2}th\\text{ term}}{2} \\right] & \\text{if } n \\text{ is even}. \\end{array} \\right. \\end{equation*} = l+\\frac{\\frac{n}{2}-C}{f} \\times d$ \n",
    "\n",
    "Mode $ = \\displaystyle l+\\frac{f_m-f_{m-1}}{2f_m-f_{m-1}-f_{m+1}}\\times d $\n",
    "\n",
    "Mode = 3Median - 2Mean\n",
    "\n",
    "Mean - Mode = 3 ( Mean - Median )\n",
    "\n",
    "variance $=\\begin{equation*} var(x)=\\sigma^2 = \\displaystyle\\frac{\\displaystyle \\sum_{i=1}^n (x_{\\tiny{i}} - \\bar{x})^2}{n} = \\displaystyle\\frac{\\displaystyle \\sum_{i=1}^n f_{\\tiny{i}}(x_{\\tiny{i}} - \\bar{x})^2}{\\displaystyle \\sum_{i=1}^n x_{\\tiny{i}}} \\end{equation*}$\n",
    "\n",
    "Standard Deviation = $ \\displaystyle\\sigma = \\sqrt{\\text{variance}} = \\sqrt{\\frac{\\sum(x_{\\tiny{i}} - \\bar{x})^2}{n}}$"
   ]
  },
  {
   "cell_type": "markdown",
   "id": "13d763e5-7619-496a-af85-bdf265a5dc2e",
   "metadata": {},
   "source": [
    "## Indices\n",
    "\n",
    "$ \\qquad\\displaystyle \\begin{aligned}\n",
    "x^m \\times x^n &= x^{m+n} \\\\  \n",
    "\\left(x^m \\right)^n &= x^{m \\times n} \\\\\n",
    "\\frac{x^m}{x^n} &= x^{m-n} \\\\\n",
    "\\left(\\frac{x}{y}\\right)^n &= \\frac{x^n}{y^n} \\\\\n",
    "x^{-n} &= \\frac{1}{x^n} \\\\\n",
    "x^0 &= 1 \\\\\n",
    "x^{\\frac{1}{n}} &= \\sqrt[n]{x} \\\\\n",
    "\\sqrt[m]{xy} &= \\sqrt[m]{x} \\times \\sqrt[m]{y} \\\\\n",
    "\\sqrt[m]{\\frac{x}{y}} &= \\frac{\\sqrt[m]{x}}{\\sqrt[m]{y}}  \\\\\n",
    "x^{\\frac{m}{n}} &= \\sqrt[n]{x^m} \\\\\n",
    "\\sqrt[m]{\\sqrt[n] {x}} &= \\sqrt[m\\times n]{x}\n",
    "\\end{aligned} $"
   ]
  },
  {
   "cell_type": "markdown",
   "id": "af244e4c-84ba-4a3b-9aee-5a60bc82d210",
   "metadata": {},
   "source": [
    "## Polygons\n",
    "\n",
    "Exterior angle + Interior angle $= 180^\\circ$\n",
    "\n",
    "Exterior angle $\\times \\ n \\text{ no. of sides} = 360^\\circ$\n",
    "\n",
    "Sum of Interior angles $ =  (n \\text{ no. of sides}-2)\\times 180^\\circ$"
   ]
  },
  {
   "cell_type": "markdown",
   "id": "8e09bc9d-c265-4bb3-a5d0-89097ff08cc4",
   "metadata": {},
   "source": [
    "\n",
    "## Euler's Equations\n",
    "\n",
    "$\\displaystyle{\\begin{align} e^{i\\theta} &= \\cos\\theta+i\\sin\\theta \\\\ e^{-i\\theta} &= \\cos\\theta-i\\sin\\theta \\\\ \\cos\\theta &= \\frac{1}{2}\\big(e^{i\\theta} + e^{-i\\theta}\\big) \\\\ \\sin\\theta &= \\frac{1}{2i}\\big(e^{i\\theta} - e^{-i\\theta}\\big) \\\\ \\tan\\theta &= \\frac{\\sin\\theta}{\\cos\\theta}=\\frac{\\big(e^{i\\theta} - e^{-i\\theta}\\big)}{i \\big(e^{i\\theta} + e^{-i\\theta}\\big)}\\end{align}}$"
   ]
  },
  {
   "cell_type": "markdown",
   "id": "4cf92fd2-3032-4175-8279-90a9c8f31cef",
   "metadata": {},
   "source": [
    "## Trigonometric Table\n",
    "\n",
    "$$\n",
    "\\begin{array}{|c|c|c|c|c|c|c|c|c|c|c|c|c|c|c|c|c|c|}\n",
    "\\hline\n",
    "\\theta (\\text{deg}) & 0^\\circ & 30^\\circ & 45^\\circ & 60^\\circ & 90^\\circ & 120^\\circ & 135^\\circ & 150^\\circ & 180^\\circ & 210^\\circ & 225^\\circ & 240^\\circ & 270^\\circ & 300^\\circ & 315^\\circ & 330^\\circ & 360^\\circ \\\\\n",
    "\\hline\n",
    "\\theta (\\text{rad}) & 0 & \\frac{\\pi}{6} & \\frac{\\pi}{4} & \\frac{\\pi}{3} & \\frac{\\pi}{2} & \\frac{2\\pi}{3} & \\frac{3\\pi}{4} & \\frac{5\\pi}{6} & \\pi & \\frac{7\\pi}{6} & \\frac{5\\pi}{4} & \\frac{4\\pi}{3} & \\frac{3\\pi}{2} & \\frac{5\\pi}{3} & \\frac{7\\pi}{4} & \\frac{11\\pi}{6} & 2\\pi \\\\\n",
    "\\hline\n",
    "\\sin\\theta & 0 & \\frac{1}{2} & \\frac{1}{\\sqrt{2}} & \\frac{\\sqrt{3}}{2} & 1 & \\frac{\\sqrt{3}}{2} & \\frac{1}{\\sqrt{2}} & \\frac{1}{2} & 0 & -\\frac{1}{2} & -\\frac{1}{\\sqrt{2}} & -\\frac{\\sqrt{3}}{2} & -1 & -\\frac{\\sqrt{3}}{2} & -\\frac{1}{\\sqrt{2}} & -\\frac{1}{2} & 0 \\\\\n",
    "\\hline\n",
    "\\cos\\theta & 1 & \\frac{\\sqrt{3}}{2} & \\frac{1}{\\sqrt{2}} & \\frac{1}{2} & 0 & -\\frac{1}{2} & -\\frac{1}{\\sqrt{2}} & -\\frac{\\sqrt{3}}{2} & -1 & -\\frac{\\sqrt{3}}{2} & -\\frac{1}{\\sqrt{2}} & -\\frac{1}{2} & 0 & \\frac{1}{2} & \\frac{1}{\\sqrt{2}} & \\frac{\\sqrt{3}}{2} & 1 \\\\\n",
    "\\hline\n",
    "\\tan\\theta & 0 & \\frac{1}{\\sqrt{3}} & 1 & \\sqrt{3} & \\infty & -\\sqrt{3} & -1 & -\\frac{1}{\\sqrt{3}} & 0 & \\frac{1}{\\sqrt{3}} & 1 & \\sqrt{3} & \\infty & -\\sqrt{3} & -1 & -\\frac{1}{\\sqrt{3}} & 0 \\\\\n",
    "\\hline\n",
    "\\csc\\theta & \\infty & 2 & \\sqrt{2} & \\frac{2}{\\sqrt{3}} & 1 & \\frac{2}{\\sqrt{3}} & \\sqrt{2} & 2 & \\infty & -2 & -\\sqrt{2} & -\\frac{2}{\\sqrt{3}} & -1 & -\\frac{2}{\\sqrt{3}} & -\\sqrt{2} & -2 & \\infty \\\\\n",
    "\\hline\n",
    "\\sec\\theta & 1 & \\frac{2}{\\sqrt{3}} & \\sqrt{2} & 2 & \\infty & 2 & \\sqrt{2} & \\frac{2}{\\sqrt{3}} & 1 & -\\frac{2}{\\sqrt{3}} & -\\sqrt{2} & -2 & \\infty & 2 & \\sqrt{2} & \\frac{2}{\\sqrt{3}} & 1 \\\\\n",
    "\\hline\n",
    "\\cot\\theta & \\infty & \\sqrt{3} & 1 & \\frac{1}{\\sqrt{3}} & 0 & -\\frac{1}{\\sqrt{3}} & -1 & -\\sqrt{3} & \\infty & \\sqrt{3} & 1 & \\frac{1}{\\sqrt{3}} & 0 & -\\frac{1}{\\sqrt{3}} & -1 & -\\sqrt{3} & \\infty \\\\\n",
    "\\hline\n",
    "\\end{array}\n",
    "$$"
   ]
  },
  {
   "cell_type": "markdown",
   "id": "2e9bbc47-b1a1-43fb-81f2-583fdc6f7b7b",
   "metadata": {},
   "source": [
    "## the angle sum identity of trigonometry\n",
    "\n",
    "$ \\displaystyle{\\sin^2 x + \\cos^2 x = 1}$                                                                                                                     \n",
    "$ \\displaystyle{\\tan^2 x + 1 = \\sec^2 x}$                                                                                                                     \n",
    "$ \\displaystyle{1 + \\cot^2 x = \\text{cosec}^2 x}$                                                                                                                     \n",
    "$ \\displaystyle{\\cos(\\alpha\\pm\\beta)=\\cos\\alpha\\cos\\beta\\mp\\sin\\alpha\\sin\\beta => \\left\\{\\begin{array}{rl} \\cos(\\alpha + \\beta)=\\cos\\alpha\\cos\\beta - \\sin\\alpha\\sin\\beta \\\\ \\cos(\\alpha - \\beta)=\\cos\\alpha\\cos\\beta + \\sin\\alpha\\sin\\beta \\end{array} \\right.  }$                                                                             \n",
    "\n",
    "$ \\displaystyle{\\sin(\\alpha\\pm\\beta)=\\sin\\alpha\\cos\\beta\\pm\\cos\\alpha\\sin\\beta => \\left\\{\\begin{array}{rl} \\sin(\\alpha + \\beta)=\\sin\\alpha\\cos\\beta + \\cos\\alpha\\sin\\beta \\\\ \\sin(\\alpha - \\beta)=\\sin\\alpha\\cos\\beta - \\cos\\alpha\\sin\\beta \\end{array} \\right.  }$                                                                                       \n",
    "\n",
    "$ \\displaystyle{\\tan(\\alpha\\pm\\beta)=\\frac{\\tan\\alpha\\pm\\tan\\beta}{1\\mp\\tan\\alpha\\tan\\beta}  => \\left\\{\\begin{array}{rl}  \\tan(\\alpha + \\beta)=\\frac{\\tan\\alpha + \\tan\\beta}{1 - \\tan\\alpha\\tan\\beta} \\\\ \\tan(\\alpha - \\beta)=\\frac{\\tan\\alpha - \\tan\\beta}{1 + \\tan\\alpha\\tan\\beta} \\end{array} \\right.  }$             \n",
    "\n",
    "\n",
    "$ \\displaystyle{\\sin(2x)=2\\sin x \\cos x=\\frac{2\\tan x}{1+\\tan^2 x}}$                                                                                                                     \n",
    "$ \\displaystyle{\\cos(2x)= \\cos^2 x - \\sin^2 x = 1-2\\sin^2 x = 2\\cos^2 x - 1 = \\frac{1-\\tan^2 x}{1+\\tan^2 x} }$                                                                                                                     \n",
    "$ \\displaystyle{\\tan(2x)=\\frac{\\sin 2x}{\\cos 2x}  =\\frac{2\\tan x}{1-\\tan^2 x} }$                                                                                                                     \n",
    "$ \\displaystyle{\\sin^2 x= \\frac{1-\\cos 2x}{2} }$                                                                                                                     \n",
    "$ \\displaystyle{\\cos^2 x= \\frac{1+\\cos 2x}{2} }$                                                                                                                     \n",
    "$ \\displaystyle{\\tan^2 x= \\frac{1-\\cos 2x}{1+\\cos 2x} }$                                                                                                                     \n",
    "$ \\displaystyle{\\sin(3x)=3\\sin x - 4\\sin^3 x}$                                                                                                                     \n",
    "$ \\displaystyle{\\cos(3x)=4\\cos^3 x - 3\\cos x}$                                                                                                                     \n",
    "$ \\displaystyle{\\tan(3x)=\\frac{\\sin 3x}{\\cos 3x}  = \\frac{3\\tan x - \\tan^3 x}{1 - 3\\tan^2 x} }$                                                             \n",
    "$ \\displaystyle{\\sin^3 x=\\frac{3\\sin x - \\sin 3x}{4}}$                                                                                                   \n",
    "$ \\displaystyle{\\cos^3 x=\\frac{\\cos 3x - 3\\cos x}{4}}$                                                                                                       \n",
    "$ \\displaystyle{\\tan^3 x=3\\tan x -\\tan(3x)( 1 - 3\\tan^2 x)}$"
   ]
  },
  {
   "cell_type": "markdown",
   "id": "353c843e-1030-49f7-9caa-df78aa644fc3",
   "metadata": {},
   "source": [
    "## Vector\n",
    "\n",
    "Del Operator  : $\\displaystyle{\\nabla \\equiv \\Big( \\frac{\\partial}{\\partial x}\\hat{i} + \\frac{\\partial}{\\partial y}\\hat{j} + \\frac{\\partial}{\\partial z}\\hat{k} \\Big)}$\n",
    "\n",
    "\n",
    "$$\n",
    "\\begin{array}{|c|c|}\n",
    "\\hline\n",
    "\\textbf{Gradient of the scalar field } \\phi\\quad\\mathrm{grad }\\ \\phi & \n",
    "\\displaystyle{\\vec{\\nabla}\\phi= \\left( \\frac{\\partial\\phi}{\\partial x}\\hat{i} + \\frac{\\partial\\phi}{\\partial y}\\hat{j} + \\frac{\\partial\\phi}{\\partial z}\\hat{k} \\right)} \\\\\n",
    "\\hline\n",
    "\\textbf{Divergence of the vector field } \\vec{f}\\quad\\mathrm{div }\\ f & \n",
    "\\displaystyle{\\vec{\\nabla}\\cdot\\vec{f}= \\left( \\frac{\\partial f_x}{\\partial x} + \\frac{\\partial f_y}{\\partial y} + \\frac{\\partial f_z}{\\partial z} \\right)} \\\\\n",
    "\\hline\n",
    "\\textbf{Curl of the vector field } \\vec{f}\\quad\\mathrm{curl }\\ f & \n",
    "\\displaystyle{\\vec{\\nabla}\\times\\vec{f}=\n",
    "\\begin{vmatrix} \n",
    "\\hat{i} & \\hat{j} & \\hat{k} \\\\\n",
    "\\frac{\\partial}{\\partial x} & \\frac{\\partial}{\\partial y} & \\frac{\\partial}{\\partial z} \\\\\n",
    "f_x & f_y & f_z \n",
    "\\end{vmatrix}} \\\\\n",
    "\\hline\n",
    "\\end{array}\n",
    "$$\n",
    "\n",
    "\n",
    "\n",
    "$\\small\\displaystyle{\\begin{align} \\nabla f &= \\hat{x}\\frac{\\partial f}{\\partial x} + \\hat{y}\\frac{\\partial f}{\\partial y} + \\hat{z}\\frac{\\partial f}{\\partial z} \\qquad\\qquad\\quad\\quad \\text{Cartesian } \\\\ &= \\hat{r}\\frac{\\partial f}{\\partial r} + \\hat{\\theta}\\frac{1}{r}\\frac{\\partial f}{\\partial \\theta} + \\hat{\\phi}\\frac{1}{r\\sin\\theta}\\frac{\\partial f}{\\partial \\phi} \\qquad\\text{spherical polars} \\\\ &= \\hat{\\rho}\\frac{\\partial f}{\\partial \\rho} + \\hat{\\phi}\\frac{1}{\\rho}\\frac{\\partial f}{\\partial \\phi} + \\hat{z}\\frac{\\partial f}{\\partial z} \\qquad\\qquad \\quad \\text{cylindrical polars} \\end{align}}$ \n",
    "\n",
    "$\\small\\displaystyle{\\begin{align} \\nabla\\times A &= \\hat{x}\\bigg(\\frac{\\partial}{\\partial y}A_z - \\frac{\\partial}{\\partial z}A_y \\bigg) + \\hat{y}\\bigg(\\frac{\\partial}{\\partial z}A_x - \\frac{\\partial}{\\partial x}A_z \\bigg) + \\hat{z}\\bigg(\\frac{\\partial}{\\partial x}A_y - \\frac{\\partial}{\\partial y}A_x \\bigg) \\qquad\\qquad\\qquad\\qquad\\qquad\\quad\\quad\\qquad \\ \\text{ Cartesian } \\\\ &= \\hat{r}\\frac{1}{r\\sin\\theta}\\bigg[ \\frac{\\partial}{\\partial\\theta}(\\sin\\theta A_{\\phi})-\\frac{\\partial}{\\partial \\phi}A_{\\theta}\\bigg] + \\hat{\\theta}\\bigg[ \\frac{1}{r\\sin\\theta}\\frac{\\partial}{\\partial\\phi}A_r-\\frac{1}{r}\\frac{\\partial}{\\partial r}(rA_{\\phi})\\bigg] + \\hat{\\phi}\\frac{1}{r}\\bigg[\\frac{\\partial}{\\partial r}(rA_{\\theta})-\\frac{\\partial}{\\partial\\theta}A_r \\bigg]\\qquad \\text{ spherical polars} \\\\ &= \\hat{\\rho}\\bigg[\\frac{1}{\\rho}\\frac{\\partial}{\\partial\\phi}A_z - \\frac{\\partial}{\\partial z}A_{\\phi} \\bigg] + \\hat{\\phi}\\bigg[\\frac{\\partial}{\\partial z}A_{\\rho} - \\frac{\\partial}{\\partial\\rho}A_z\\bigg] + \\hat{z}\\frac{1}{\\rho}\\bigg[\\frac{\\partial}{\\partial\\rho}(\\rho A_{\\phi}) - \\frac{\\partial}{\\partial\\phi}A_{\\rho}  \\bigg] \\qquad\\qquad\\qquad\\qquad\\qquad\\qquad  \\text{cylindrical polars} \\end{align}}$  \n",
    "\n",
    "$\\small\\displaystyle{\\begin{align} \\nabla\\cdot A &= \\frac{\\partial}{\\partial x}A_x + \\frac{\\partial}{\\partial y}A_y + \\frac{\\partial}{\\partial z}A_z \\qquad\\qquad\\qquad\\qquad\\qquad\\qquad\\qquad \\text{Cartesian } \\\\ &= \\frac{1}{r^2}\\frac{\\partial}{\\partial r}(r^2A_r) + \\frac{1}{r\\sin\\theta}\\frac{\\partial}{\\partial\\theta}(\\sin\\theta A_{\\theta}) + \\frac{1}{r\\sin\\theta}\\frac{\\partial}{\\partial\\phi}A_{\\phi} \\qquad\\quad\\text{spherical polars} \\\\ &= \\frac{1}{\\rho} \\frac{\\partial}{\\partial \\rho}(\\rho A_{\\rho}) + \\frac{1}{\\rho}\\frac{\\partial}{\\partial\\phi}A_{\\phi} + \\frac{\\partial}{\\partial z}A_z \\qquad\\qquad\\qquad\\qquad \\quad\\qquad \\text{cylindrical polars} \\end{align}}$         \n",
    "\n",
    "$\\small\\displaystyle{\\begin{align} \\nabla^2f &= \\frac{\\partial^2 f}{\\partial x^2} + \\frac{\\partial^2 f}{\\partial y^2} + \\frac{\\partial^2 f}{\\partial z^2} \\qquad\\qquad\\qquad\\qquad\\qquad\\qquad\\qquad\\qquad \\text{Cartesian } \\\\\n",
    "&= \\frac{1}{r}\\frac{\\partial^2}{\\partial r^2}(rf) + \\frac{1}{r^2\\sin\\theta}\\frac{\\partial }{\\partial \\theta}\\bigg(\\sin\\theta\\frac{\\partial f}{\\partial\\theta}\\bigg) + \\frac{1}{r^2\\sin^2\\theta}\\frac{\\partial^2 f}{\\partial \\phi^2} \\qquad\\text{spherical polars} \\\\ &= \\frac{1}{\\rho}\\frac{\\partial}{\\partial \\rho}\\bigg(\\rho\\frac{\\partial f}{\\partial \\rho}\\bigg) + \\frac{1}{\\rho^2}\\frac{\\partial^2 f}{\\partial \\phi^2} + \\frac{\\partial^2 f}{\\partial z^2} \\qquad\\qquad\\qquad\\qquad\\quad\\qquad \\text{cylindrical polars} \\end{align}}$                                          "
   ]
  }
 ],
 "metadata": {
  "kernelspec": {
   "display_name": "Python 3 (ipykernel)",
   "language": "python",
   "name": "python3"
  },
  "language_info": {
   "codemirror_mode": {
    "name": "ipython",
    "version": 3
   },
   "file_extension": ".py",
   "mimetype": "text/x-python",
   "name": "python",
   "nbconvert_exporter": "python",
   "pygments_lexer": "ipython3",
   "version": "3.11.0"
  }
 },
 "nbformat": 4,
 "nbformat_minor": 5
}
